Disjoint.v
@@ -53,11 +53,12 @@ Set Printing All.
  * provide construction to get elem of type in opt_loop_CFG
  * this is the element to instantiate in the path_splits__imp definition. *)
 
+(*
 Lemma in_implode_CFG (* unused *)`{C : redCFG} (p : Lab)
       (Hdeq : deq_loop root p)
   : implode_nodes C p.
 Admitted.
-  
+ *)
 
 Arguments loop_head {_ _ _ _} _.
 Arguments loop_head_dec {_ _ _ _} _.
@@ -89,12 +90,13 @@ Admitted.
 Lemma head_exits_exited_inv `(C : redCFG) (h p : Lab)
   : exited C h p <-> exited (head_exits_CFG C) h p.
 Admitted.
-Lemma head_exits_deq_loop_inv `(C : redCFG) (p q : Lab)
-  : deq_loop C p q <-> deq_loop (head_exits_CFG C) p q.
+Lemma head_exits_deq_loop_inv1 `(C : redCFG) (p q : Lab)
+  : deq_loop C p q -> deq_loop (head_exits_CFG C) p q.
 Admitted.
 Lemma head_exits_depth_inv (* unused *)`(C : redCFG) (p : Lab)
   : depth C p = depth (head_exits_CFG C) p.
-Admitted.  
+Admitted.
+(*
 Lemma no_strictly_containing_loop_impl_top_level:
   forall (Lab : finType) (edge : Lab -> Lab -> bool) (root : Lab) (a_edge : Lab -> Lab -> bool)
     (C : redCFG edge root a_edge) (p : Lab),
@@ -103,47 +105,42 @@ Lemma no_strictly_containing_loop_impl_top_level:
 Proof.
   intros.
 Admitted.
-
+*)
 Definition thrice (A B : Type) (f : A -> B) (xyz : A*A*A) : B*B*B
   := match xyz with (x,y,z) => (f x, f y, f z) end.
 
+
+Definition get_innermost_loop' `{C : redCFG} p
+  := match get_innermost_loop p with
+     | Some (exist _ h _) => h
+     | None => root
+     end.
+
+Lemma deq_loop_innermost' `{C : redCFG} (p : Lab)
+  : deq_loop C (get_innermost_loop' p) p.
+Proof.
+  remember (get_innermost_loop' p) as h.
+  specialize (get_innermost_loop_spec p) as Hspec.
+  unfold get_innermost_loop' in Heqh.
+  destruct (get_innermost_loop p).
+  - destruct s. subst. unfold innermost_loop in Hspec. subst. destructH; auto.
+  - subst. unfold deq_loop. intros. exfalso; eauto.
+Qed.   
+    
+
 Program Definition path_splits__imp' `{C : redCFG} (p : Lab)
-  := let d := (option_map (loop_containsT_loop_head (C:=C) (p:=p))
-                          (get_innermost_loop_strict C p)) in
-     let D := (local_impl_CFG C d) in
+  := let D := (local_impl_CFG C (get_innermost_loop' p)) in
      (@path_splits _ _ _ _ D _).
 Next Obligation.
   eapply implode_CFG_elem.
-  Unshelve.
-  all:cycle 1.
-  {
-    set (d:=(option_map (loop_containsT_loop_head (p:=p)) (get_innermost_loop_strict C p))).
-    eapply (opt_loop_CFG_elem).
-    destruct d eqn:E;[|exact I].
-    unfold option_map in *.
-    subst d. destruct (get_innermost_loop_strict C p);inversion E.
-    subst s.
-    destruct s0. cbn in *. eauto.
-  }  
-  unfold implode_nodes. unfold predicate.
-  match goal with [|- deq_loop _ ?rr ?pp \/ _] => set (root':=rr); set (p':=pp) end. cbn in root', p'.
-  specialize (get_innermost_loop_strict_spec p) as Hspec.
-  rewrite <-head_exits_deq_loop_inv.
-  setoid_rewrite <-head_exits_deq_loop_inv.
-  setoid_rewrite <-head_exits_exited_inv.
-  destruct (get_innermost_loop_strict C p) eqn:E; cbn in root', p'.
-  - unfold option_map, opt_loop_CFG. unfold loop_containsT_loop_head. destruct s. cbn in p'. cbn in root'.
-    eapply (loop_CFG_top_level);eauto. 
-  - unfold option_map, opt_loop_CFG. subst root' p'.
-    eapply no_strictly_containing_loop_impl_top_level;auto.
+  left. eapply head_exits_deq_loop_inv1. 
+  eapply deq_loop_innermost'. 
 Defined.
 
 Arguments exited {_ _ _ _ _} _.
 
 Definition path_splits__imp `{C : redCFG} (p : Lab)
-  := let d := (option_map (loop_containsT_loop_head (C:=C) (p:=p))
-                          (get_innermost_loop_strict C p)) in
-     map (thrice (original_of_impl (d:=d))) (path_splits__imp' p).
+  := map (thrice (@proj1_sig Lab _)) (path_splits__imp' p).
 
 Lemma exited_head (* unused *)`{C : redCFG} (h e : Lab)
       (H : exited h e)
@@ -152,46 +149,30 @@ Proof.
   unfold exited in H. destructH. unfold exit_edge in H. destructH. eapply loop_contains_loop_head;eauto.
 Qed.
 
-Definition loop_splits__imp' `{C : redCFG} (h e : Lab)
-  := let d := match decision (loop_head C h) with
-              | left H => Some (exist _ h H)
-              | right _ => None
-              end in
-    match impl_of_original d h, impl_of_original d e with
-    | Some h', Some e' => (@loop_splits _ _ _ _ (local_impl_CFG C d)
-                                       h' e')
-    | _,_ => nil
-    end.
+Program Definition loop_splits__imp' `{C : redCFG} (h e : Lab)
+  := match decision (exited h e) with
+     | left H => (@loop_splits _ _ _ _ (local_impl_CFG C h) _ _)
+     | _ => nil
+     end.
+Next Obligation.
+  eapply implode_CFG_elem.
+  left. eapply head_exits_deq_loop_inv1.
+  eapply deq_loop_refl.
+Defined.
+Next Obligation.
+  eapply implode_CFG_elem.
+  left. eapply head_exits_deq_loop_inv1.
+  unfold exited in H. destructH.
+  eapply deq_loop_exited';eauto.
+Defined.
+
 
 Definition loop_splits__imp `{C : redCFG} (h e : Lab)
   := let d := match decision (loop_head C h) with
               | left H => Some (exist _ h H)
               | right _ => None
               end in
-     map (thrice (original_of_impl (d:=d))) (loop_splits__imp' h e).
-(*Next Obligation.
-  eapply implode_CFG_elem.
-  Unshelve.
-  all:cycle 1.
-  {
-    eapply (opt_loop_CFG_elem). 
-    decide (loop_head C h);[|exact I].
-    eapply loop_contains_self;eauto.
-  } 
-  unfold implode_nodes. unfold predicate.
-  match goal with [|- deq_loop _ ?rr ?pp \/ _] => set (root':=rr); set (p':=pp) end. cbn in root', p'.
-  rewrite <-head_exits_head_inv.
-  rewrite <-head_exits_deq_loop_inv.
-  do 2 rewrite <-head_exits_depth_inv.
-  decide (loop_head C h);cbn in root', p'; subst root' p';unfold opt_loop_CFG.
-  - left. unfold deq_loop. cbn. eauto. admit.
-  - 
-  destruct (get_innermost_loop_strict C h) eqn:E; cbn in root', p'.
-  - unfold option_map, opt_loop_CFG. unfold loop_containsT_loop_head. destruct s. cbn in p'. cbn in root'.
-    eapply (loop_CFG_top_level);eauto. 
-  - unfold option_map, opt_loop_CFG. subst root' p'.
-    eapply no_strictly_containting_loop_impl_top_level;auto.
-Defined.*)
+     map (thrice (@proj1_sig Lab _)) (loop_splits__imp' h e).
 
 Parameter splits'_spec (* unused *)
   : forall `{redCFG} h e sp, sp ∈ splits' h e
@@ -286,7 +267,7 @@ Definition get_innermost_loop_strict' `{C : redCFG} p
      | Some (exist _ h _) => h
      | None => root
      end.
-
+(*
 Lemma impl_list_cfg_tpath (* unused *)`{C : redCFG} l p i
       (Hin : forall q, q ∈ map fst l -> loop_contains (get_innermost_loop_strict' p) q)
       (Hpath : TPath' ((p,i) :< l))
@@ -294,6 +275,7 @@ Lemma impl_list_cfg_tpath (* unused *)`{C : redCFG} l p i
   : TPath' ((p,i) :< impl_list' p l).
 Proof.
 Admitted.
+ *)
 
 Lemma impl_disj_coord_impl_disj_lab `{redCFG} l1 l2 s p i
       (Hpath1 : TPath' ((p,i) :< l1 :>: (s,i)))
@@ -454,7 +436,8 @@ Proof.
     eapply lc_join_path_split in Hlc;eauto.
     destructH.
     eexists; eexists. eapply splits_spec. left. eauto.
-  -  
+  - eapply lc_implode_in in Htri;cycle 2;eauto. admit.
+    destructH.
 Admitted.
 
 
